$$
J=D+C .11^{T}
$$

where,

$$
\begin{aligned}
& D=\operatorname{diag}\left\{1 / \alpha_{1}, \ldots, 1 / \alpha_{k-1}\right\} \\
& C=\frac{1}{1-\sum_{j=1}^{k-1} \alpha_{j}}
\end{aligned}
$$

Goal is to find $J^{-1}$
[General formula: $\left(A+\underset{\sim}{u} \underset{\sim}{v}{ }^{\top}\right)^{-1}$

$$
\begin{aligned}
& \left.=A^{-1}-\frac{A^{-1} \underset{\sim}{u}{\underset{\sim}{v}}^{\top} A^{-1}}{\left(1+\underset{\sim}{v} A^{\top} \underline{u}\right)}\right] \\
& J^{-1}=D^{-1}-\frac{D^{-1} c \perp \perp^{\top} D^{-1}}{\left(1+c \perp^{\top} D^{-1} \perp\right)} \\
& {[\underset{\sim}{u}=c 1} \\
& \underset{\sim}{v}=1] \\
& =\left(\begin{array}{llll}
\alpha_{1} & & \\
& & & \\
& & & \\
& & \alpha_{k-1}
\end{array}\right) \\
& -e \cdot\left(\begin{array}{c}
\alpha_{1} \\
\vdots \\
\alpha_{k-1}
\end{array}\right)\left(\alpha_{1} \ldots \alpha_{k-1}\right) \\
& {\left[I^{\top} D^{-1} \stackrel{1}{\sim}\right.} \\
& =\mathcal{L}^{\top}\left(\alpha_{1} \cdot{ }^{k-1} \alpha_{k-1}\right)^{-1} \perp \\
& \left.=\sum_{i=1}^{k-1} \alpha_{i}\right] \\
& e=\frac{c}{1+c \sum_{i=1}^{k-1} \alpha_{i}} \\
& =\frac{\frac{1}{1-\sum_{i=1}^{k-1} \alpha_{i}}}{1+\frac{\sum_{i=1}^{k-1} \alpha_{i}}{1-\sum_{i=1}^{k-1} \alpha_{i}}}=1 \\
& J^{-1}=\left(\begin{array}{llll}
\alpha_{1} & & & \\
& \ddots & \\
& & \ddots \alpha_{k-1}
\end{array}\right)-\left(\begin{array}{cc}
\alpha_{1} \\
\vdots \\
\alpha_{k-1}
\end{array}\right)\left(\begin{array}{ll}
\alpha_{1} & \ldots \alpha_{k-1}
\end{array}\right)
\end{aligned}
$$

